storage_ops_solvers_impl_soundness.v
@@ -1,8 +1,9 @@
 Require Import Arith.   
-Require Import Nat. 
+Require Import Nat.  
 Require Import Bool.
 Require Import bbv.Word.
 Require Import Coq.NArith.NArith.
+Require Import Coq.NArith.Nnat.
 Require Import List.
 Import ListNotations.
 Require Import Coq.Logic.FunctionalExtensionality.
@@ -30,7 +31,7 @@ Import SymbolicStateEval.
 
 Require Import FORVES.symbolic_state_eval_facts.
 Import SymbolicStateEvalFacts.
-
+ 
 Require Import FORVES.valid_symbolic_state.
 Import ValidSymbolicState.
 
@@ -40,6 +41,11 @@ Import StorageOpsSolvers.
 Require Import FORVES.storage_ops_solvers_impl.
 Import StorageOpsSolversImpl.
 
+Require Import FORVES.symbolic_execution_soundness.
+Import SymbolicExecutionSoundness.
+
+Require Import FORVES.sstack_val_cmp_impl_soundness.
+Import SStackValCmpImplSoundness.
 Module StorageOpsSolversImplSoundness.
 
  
@@ -111,7 +117,131 @@ Module StorageOpsSolversImplSoundness.
       repeat split; apply H_eval_sstorage_u_sstrg.
   Qed.
   
-        
+  Lemma not_eq_keys_snd:
+    forall skey skey' maxidx sbindings instk_height ops,
+      valid_bindings instk_height maxidx sbindings ops ->
+      valid_sstack_value instk_height maxidx skey ->
+      valid_sstack_value instk_height maxidx skey' ->
+      not_eq_keys skey skey' maxidx sbindings instk_height ops = true ->
+      forall stk mem strg ctx,
+        (length stk) = instk_height ->
+        exists v1 v2,
+        eval_sstack_val' (S maxidx) skey stk mem strg ctx maxidx sbindings ops = Some v1 /\
+          eval_sstack_val' (S maxidx) skey' stk mem strg ctx maxidx sbindings ops = Some v2 /\
+          weqb v1 v2 = false.
+  Proof.
+    intros skey skey' maxidx sbindings instk_height ops.
+    intros H_valid_bs H_valid_skey H_valid_skey' H_neq.
+    unfold not_eq_keys in H_neq.
+    destruct (follow_in_smap skey maxidx sbindings) as [skey_m|] eqn:E_follow_skey; try discriminate.
+    destruct skey_m; try discriminate.
+    destruct smv; try discriminate.
+    destruct val; try discriminate.
+    destruct (follow_in_smap skey' maxidx sbindings) as [skey'_m|] eqn:E_follow_skey'; try discriminate.
+    destruct skey'_m; try discriminate.
+    destruct smv; try discriminate.
+    destruct val0; try discriminate.
+    intros stk mem strg ctx.
+    intros H_stk_len.
+    unfold eval_sstack_val' at 1.
+    rewrite E_follow_skey.
+    unfold eval_sstack_val' at 1.
+    rewrite E_follow_skey'.
+    exists val.
+    exists val0.
+    split; try split; try reflexivity.
+    rewrite negb_true_iff in H_neq.
+    rewrite H_neq.
+    reflexivity.
+Qed.      
+                                                                                             
+Lemma H_map_o_sstrg:
+  forall instk_height d stk mem strg ctx maxidx bs ops sstrg,
+    valid_sstorage instk_height maxidx sstrg ->
+    valid_bindings instk_height maxidx bs ops ->
+    d > maxidx ->
+    instk_height = length stk ->
+    exists v,
+      map_option (eval_common.EvalCommon.instantiate_storage_update (fun sv : sstack_val => eval_sstack_val' d sv stk mem strg ctx maxidx bs ops)) sstrg = Some v.
+Proof.
+induction sstrg as [|u sstrg' IHsstrg'].
++ intros. simpl. exists []. reflexivity.
++ intros H_valid_sstorage H_valid_bs H_d_gt_maxidx H_len_stk.
+  unfold map_option.
+  rewrite <- map_option_ho.
+  unfold eval_common.EvalCommon.instantiate_storage_update at 1.
+  destruct u as [skey' svalue'].
+                            
+  unfold valid_sstorage in H_valid_sstorage. fold valid_sstorage in H_valid_sstorage.
+  destruct H_valid_sstorage as [H_valid_sstorage_0 H_valid_sstorage_1].
+  unfold valid_sstorage_update in H_valid_sstorage_0.
+  destruct H_valid_sstorage_0 as [H_valid_sstorage_0_0 H_valid_sstorage_0_1].
+
+  pose proof (eval_sstack_val'_succ d instk_height skey' stk mem strg ctx maxidx bs ops H_len_stk H_valid_sstorage_0_0 H_valid_bs H_d_gt_maxidx) as eval_sstack_val'_succ_0.
+  
+  destruct eval_sstack_val'_succ_0 as [v eval_sstack_val'_succ_0].
+  rewrite eval_sstack_val'_succ_0.
+  pose proof (eval_sstack_val'_succ d instk_height svalue' stk mem strg ctx maxidx bs ops H_len_stk H_valid_sstorage_0_1 H_valid_bs H_d_gt_maxidx) as eval_sstack_val'_succ_1.
+  destruct eval_sstack_val'_succ_1 as [v' eval_sstack_val'_succ_1].
+  rewrite eval_sstack_val'_succ_1.
+
+  pose proof (IHsstrg' H_valid_sstorage_1 H_valid_bs H_d_gt_maxidx H_len_stk) as IHsstrg'_0.
+  destruct IHsstrg'_0 as [v'' IHsstrg'_0].
+  rewrite IHsstrg'_0.
+  exists (U_SSTORE EVMWord v v' :: v'').
+  reflexivity.
+  Qed.
+
+Lemma ssload_sstore_same_address:
+  forall strg addr value,
+    (concrete_interpreter.ConcreteInterpreter.sload
+       (concrete_interpreter.ConcreteInterpreter.sstore strg addr value) addr) = value.
+Proof.
+  intros strg addr value.
+  unfold concrete_interpreter.ConcreteInterpreter.sstore.
+  unfold concrete_interpreter.ConcreteInterpreter.sload.
+  rewrite N.eqb_refl with (x:= (wordToN addr)).
+  reflexivity.
+Qed.  
+
+
+Lemma eval_sstack_val'_immediate_fresh_var:
+  forall d idx stk mem strg ctx value bs ops,
+  eval_sstack_val' d (FreshVar idx) stk mem strg ctx (S idx) ((idx, SymBasicVal value) :: bs) ops =
+    eval_sstack_val' d value stk mem strg ctx idx bs ops.
+Proof.
+  intros d idx stk mem strg ctx value bs ops.
+  destruct d as [|d']; try reflexivity.
+  destruct value as [v|i|i] eqn:E_value.
+  + unfold eval_sstack_val'  at 1.
+    fold eval_sstack_val'.
+    rewrite follow_smap_first_match; try reflexivity.
+    unfold eval_sstack_val'  at 1.
+    fold eval_sstack_val'.
+    rewrite follow_smap_V.
+    reflexivity.
+  + unfold eval_sstack_val'  at 1.
+    fold eval_sstack_val'.
+    rewrite follow_smap_first_match; try reflexivity.
+    unfold eval_sstack_val'  at 1.
+    fold eval_sstack_val'.
+    rewrite follow_smap_InStackVar.
+    reflexivity.
+  + unfold eval_sstack_val'  at 1.
+    fold eval_sstack_val'.
+    unfold follow_in_smap.
+    fold follow_in_smap.
+    rewrite Nat.eqb_refl.
+    unfold is_fresh_var_smv.
+    unfold eval_sstack_val'  at 9.
+    fold eval_sstack_val'.
+    reflexivity.
+Qed.    
+    
+
+  
+   
+
   Lemma basic_sload_solver_snd: sload_solver_ext_snd basic_sload_solver.
   Proof.
     unfold sload_solver_ext_snd.
@@ -152,7 +282,7 @@ Module StorageOpsSolversImplSoundness.
       induction sstrg as [| u sstrg' IH_sstrg'].
       + simpl in H_basic_sload_solver.
         rewrite <- H_basic_sload_solver in H_add_to_smap.
-        exists idx1. exists m1.        
+        exists idx1. exists m1.
         split; try auto.
         intros stk mem strg ctx H_len_stk.
         symmetry in H_len_stk.
@@ -163,21 +293,273 @@ Module StorageOpsSolversImplSoundness.
         pose proof (add_to_smap_key_lt_maxidx m m1 idx1 (SymSLOAD skey []) H_add_to_smap') as H_idx1_lt_maxidx_m1.
         pose proof (valid_sstack_val_freshvar instk_height (get_maxidx_smap m1) idx1 H_idx1_lt_maxidx_m1) as H_valid_fresh_idx1.
         unfold valid_smap in H_valid_m1.
-        pose proof (eval_sstack_val_succ (get_bindings_smap m1) instk_height (FreshVar idx1) stk mem strg ctx (get_maxidx_smap m1) ops H_len_stk H_valid_fresh_idx1 H_valid_m1) as H_eval_sstack_val.        
+        pose proof (eval_sstack_val_succ (get_bindings_smap m1) instk_height (FreshVar idx1) stk mem strg ctx (get_maxidx_smap m1) ops H_len_stk H_valid_fresh_idx1 H_valid_m1) as H_eval_sstack_val.
         destruct H_eval_sstack_val as [v H_eval_sstack_val].
         exists v.
         rewrite H_eval_sstack_val.
         split; reflexivity.
+      + unfold basic_sload_solver in H_basic_sload_solver.
+        destruct u.
+        simpl in H_valid_sstrg.
+        destruct H_valid_sstrg as [[H_valid_key H_valid_value] H_valid_sstrg'].
+        destruct (sstack_val_cmp (S (get_maxidx_smap m)) skey key (get_maxidx_smap m) (get_bindings_smap m) (get_maxidx_smap m) (get_bindings_smap m) instk_height ops) eqn:E_cmp_skey_key.
         
+        * destruct m as [maxidx_m bs_m] eqn:E_m.
+          exists maxidx_m.
+          exists (SymMap (S maxidx_m) ((maxidx_m,(SymSLOAD skey (U_SSTORE sstack_val key value :: sstrg')))::bs_m)).
+          split.
+          ++ simpl. reflexivity.
+          ++ intros stk mem strg ctx H_len_stk.
+             rewrite <- H_basic_sload_solver in H_add_to_smap.
+             simpl in H_add_to_smap.
+             injection H_add_to_smap as H_idx1 H_m1.
+             rewrite <- H_idx1.
+             rewrite <- H_m1.
+             simpl.
+             unfold eval_sstack_val.
+             rewrite eval_sstack_val'_immediate_fresh_var.
+             remember (S maxidx_m) as S_maxidx_m.
+             unfold eval_sstack_val' at 2.
+             fold eval_sstack_val'.
+             rewrite HeqS_maxidx_m.
+             rewrite follow_smap_first_match; try reflexivity.  (* the reflexivity is for is_fresh_var_smv *)
+
+             unfold symbolic_state_cmp.SymbolicStateCmp.safe_sstack_val_cmp_ext_1 in H_sstack_val_cmp_snd.
+             pose proof (H_sstack_val_cmp_snd (S maxidx_m)) as H_sstack_val_cmp_snd.
+             unfold symbolic_state_cmp.SymbolicStateCmp.safe_sstack_val_cmp_ext_1_d in H_sstack_val_cmp_snd.
+             pose proof (H_sstack_val_cmp_snd (S maxidx_m) (Nat.le_refl (S maxidx_m) )) as H_sstack_val_cmp_snd.
+             unfold symbolic_state_cmp.SymbolicStateCmp.safe_sstack_val_cmp in H_sstack_val_cmp_snd.
+             pose proof (H_sstack_val_cmp_snd skey key maxidx_m bs_m maxidx_m bs_m instk_height ops H_valid_skey H_valid_key H_valid_smap H_valid_smap E_cmp_skey_key stk mem strg ctx H_len_stk) as H_sstack_val_cmp_snd.
+             destruct H_sstack_val_cmp_snd as [v [H_sstack_val_cmp_snd_1 H_sstack_val_cmp_snd_2]].
+             unfold eval_sstack_val in H_sstack_val_cmp_snd_1.
+             unfold eval_sstack_val in H_sstack_val_cmp_snd_2.
+
+             pose proof (valid_sstorage_update_kv instk_height maxidx_m key value H_valid_key H_valid_value) as H_valid_update.
+             pose proof (valid_sstorage_when_extended_with_valid_update instk_height maxidx_m (U_SSTORE sstack_val key value) sstrg' H_valid_update H_valid_sstrg') as H_valid_u_sstrg'.
+             pose proof (H_map_o_sstrg instk_height (S maxidx_m) stk mem strg ctx maxidx_m bs_m ops (U_SSTORE sstack_val key value :: sstrg') H_valid_u_sstrg' H_valid_smap (gt_Sn_n maxidx_m) (eq_sym H_len_stk)) as H_map_o_sstrg_0.
+             destruct H_map_o_sstrg_0 as [v' H_map_o_sstrg_0].
+             rewrite H_map_o_sstrg_0.
+             rewrite H_sstack_val_cmp_snd_1.
+             destruct v'.
+             
+             +++ pose proof (map_option_len (storage_update sstack_val) (storage_update EVMWord) (eval_common.EvalCommon.instantiate_storage_update (fun sv : sstack_val => eval_sstack_val' (S maxidx_m) sv stk mem strg ctx maxidx_m bs_m ops)) (U_SSTORE sstack_val key value :: sstrg') [] H_map_o_sstrg_0) as H_l_len.
+                 discriminate.
+             +++ pose proof (map_option_hd (storage_update sstack_val) (storage_update EVMWord) (eval_common.EvalCommon.instantiate_storage_update (fun sv : sstack_val => eval_sstack_val' (S maxidx_m) sv stk mem strg ctx maxidx_m bs_m ops)) sstrg' v' (U_SSTORE sstack_val key value) s H_map_o_sstrg_0) as H_map_o_sstrg_1.
+                 destruct H_map_o_sstrg_1 as [H_map_o_sstrg_1_0 H_map_o_sstrg_1_1].
+
+                 unfold eval_common.EvalCommon.instantiate_storage_update in H_map_o_sstrg_1_0.
+                 rewrite H_sstack_val_cmp_snd_2 in H_map_o_sstrg_1_0.
+                 destruct (eval_sstack_val' (S maxidx_m) value stk mem strg ctx maxidx_m bs_m ops) as [value_v|] eqn:E_eval_value; try discriminate.
+                 pose proof (eval_sstack_val'_preserved_when_depth_extended_le (S maxidx_m) (S (S maxidx_m)) maxidx_m bs_m value value_v stk mem strg ctx ops (Nat.le_succ_diag_r (S maxidx_m)) E_eval_value) as E_eval_value_0.
+                 rewrite E_eval_value_0.
+
+                 injection H_map_o_sstrg_1_0 as H_map_o_sstrg_1_0.
+                 rewrite <- H_map_o_sstrg_1_0.
+
+                 simpl.
+                
+                 rewrite ssload_sstore_same_address.
+                 exists value_v.
+                 split; reflexivity.
+      * fold basic_sload_solver in H_basic_sload_solver.
+        destruct (not_eq_keys skey key (get_maxidx_smap m) (get_bindings_smap m) instk_height ops) eqn:E_not_eq_keys.
+        ** pose proof (IH_sstrg' H_valid_sstrg' H_basic_sload_solver) as IH_sstrg'_0.
+           destruct IH_sstrg'_0 as [idx2 IH_sstrg'_0].
+           destruct IH_sstrg'_0 as [m2 IH_sstrg'_0].
+           destruct IH_sstrg'_0 as [IH_sstrg'_0_0 IH_sstrg'_0_1].
+           destruct m eqn:E_m.
+           simpl in IH_sstrg'_0_0.
+           injection IH_sstrg'_0_0 as IH_sstrg'_0_0_0 IH_sstrg'_0_0_1.
+           simpl.
+           exists maxid.
+           exists (SymMap (S maxid) ((maxid, SymSLOAD skey (U_SSTORE sstack_val key value :: sstrg')) :: bindings)).
+           split; try reflexivity.
+           intros stk mem strg ctx H_stk_len.
+           simpl in H_add_to_smap.
+           injection H_add_to_smap as H_add_to_smap_0 H_add_to_smap_1.
+           rewrite <- H_add_to_smap_1.
+           rewrite <- H_add_to_smap_0.
+           simpl.
+           rewrite <- IH_sstrg'_0_0_1 in IH_sstrg'_0_1.
+           rewrite <- H_add_to_smap_1 in IH_sstrg'_0_1.
+           rewrite <- IH_sstrg'_0_0_0 in IH_sstrg'_0_1.
+           rewrite <- H_add_to_smap_0 in IH_sstrg'_0_1.
+           simpl in IH_sstrg'_0_1.
+           unfold eval_sstack_val.
+           unfold eval_sstack_val in IH_sstrg'_0_1.
+           remember (S maxid) as S_maxid.
+           unfold eval_sstack_val' at 2.
+           fold eval_sstack_val'.
+           rewrite HeqS_maxid.
+           rewrite follow_smap_first_match; try reflexivity.
+
+           pose proof (valid_sstorage_update_kv instk_height maxid key value H_valid_key H_valid_value) as H_valid_update.
+           pose proof (valid_sstorage_when_extended_with_valid_update instk_height maxid (U_SSTORE sstack_val key value) sstrg' H_valid_update H_valid_sstrg') as H_valid_u_sstrg'.
+           pose proof (H_map_o_sstrg instk_height (S maxid) stk mem strg ctx maxid bindings ops (U_SSTORE sstack_val key value :: sstrg') H_valid_u_sstrg' H_valid_smap (gt_Sn_n maxid) (eq_sym H_stk_len)) as H_map_o_sstrg_0.
+           destruct H_map_o_sstrg_0 as [v H_map_o_sstrg_0].
+           rewrite H_map_o_sstrg_0.
+
+           pose proof (IH_sstrg'_0_1 stk mem strg ctx H_stk_len) as IH_sstrg'_0_1_0.
+           destruct IH_sstrg'_0_1_0 as [v' IH_sstrg'_0_1_0].
+           destruct IH_sstrg'_0_1_0 as [IH_sstrg'_0_1_0_0 IH_sstrg'_0_1_0_1].
+           exists v'.
+           split.
+           *** rewrite <- HeqS_maxid.
+               apply IH_sstrg'_0_1_0_0.
+           *** pose proof (eval_sstack_val'_succ (S maxid) instk_height skey stk mem strg ctx maxid bindings ops (eq_sym H_stk_len) H_valid_skey H_valid_smap (gt_Sn_n maxid)) as H_eval_skey.
+               destruct H_eval_skey as [skey_v H_eval_skey].
+               rewrite  H_eval_skey.
+           
+               destruct v.
+             
+             +++ pose proof (map_option_len (storage_update sstack_val) (storage_update EVMWord) (eval_common.EvalCommon.instantiate_storage_update (fun sv : sstack_val => eval_sstack_val' (S maxid) sv stk mem strg ctx maxid bindings ops)) (U_SSTORE sstack_val key value :: sstrg') [] H_map_o_sstrg_0) as H_l_len.
+                 discriminate.
+             +++ pose proof (map_option_hd (storage_update sstack_val) (storage_update EVMWord) (eval_common.EvalCommon.instantiate_storage_update (fun sv : sstack_val => eval_sstack_val' (S maxid) sv stk mem strg ctx maxid bindings ops)) sstrg' v (U_SSTORE sstack_val key value) s H_map_o_sstrg_0) as H_map_o_sstrg_1.
+                 destruct H_map_o_sstrg_1 as [H_map_o_sstrg_1_0 H_map_o_sstrg_1_1].
+
+                 unfold eval_common.EvalCommon.instantiate_storage_update in H_map_o_sstrg_1_0.
+
+                 destruct (eval_sstack_val' (S maxid) key stk mem strg ctx maxid bindings ops) as [key_v|] eqn:E_eval_key; try discriminate.
+                 destruct (eval_sstack_val' (S maxid) value stk mem strg ctx maxid bindings ops) as [value_v|] eqn:E_eval_value; try discriminate.
+                 injection H_map_o_sstrg_1_0 as H_map_o_sstrg_1_0.
+                 rewrite <- H_map_o_sstrg_1_0.
+
+                 simpl.
+                 remember (eval_common.EvalCommon.update_storage strg v) as strg_w_v.
+                 unfold concrete_interpreter.ConcreteInterpreter.sstore.
+                 unfold concrete_interpreter.ConcreteInterpreter.sload.
+
+                 pose proof (not_eq_keys_snd skey key maxid bindings instk_height ops H_valid_smap H_valid_skey H_valid_key E_not_eq_keys stk mem strg ctx H_stk_len) as H_not_eq_keys_snd.
+                 destruct H_not_eq_keys_snd as [v1 [v2 [not_eq_keys_snd_0 [not_eq_keys_snd_1 not_eq_keys_snd_3]]]].
+                 rewrite H_eval_skey in not_eq_keys_snd_0.
+                 injection not_eq_keys_snd_0 as not_eq_keys_snd_0.
+                 rewrite not_eq_keys_snd_0.
+                 rewrite E_eval_key in not_eq_keys_snd_1.
+                 injection not_eq_keys_snd_1 as not_eq_keys_snd_1.
+                 rewrite not_eq_keys_snd_1.
+
+                 
+                 assert( H_v1_neq_v2:  (wordToN v1 =? wordToN v2)%N = false ).
+                 {
+                   assert( (wordToNat v1) <> (wordToNat v2)).
+                   {
+                     apply wordToNat_neq1.
+                     apply weqb_false.
+                     apply not_eq_keys_snd_3.
+                   }
+                   rewrite wordToN_nat.
+                   rewrite wordToN_nat.
+                   rewrite N.eqb_neq.
+                   intuition.
+                 }
+
+                 rewrite H_v1_neq_v2.
+                 unfold eval_sstack_val' in IH_sstrg'_0_1_0_1.
+                 fold eval_sstack_val' in IH_sstrg'_0_1_0_1.
+                 rewrite HeqS_maxid in IH_sstrg'_0_1_0_1.
+                 rewrite follow_smap_first_match in IH_sstrg'_0_1_0_1; try reflexivity.
+                 destruct (map_option (eval_common.EvalCommon.instantiate_storage_update (fun sv : sstack_val => eval_sstack_val' (S maxid) sv stk mem strg ctx maxid bindings ops)) sstrg') eqn:E_map_op_sstrg'; try discriminate.
+                 rewrite H_eval_skey in IH_sstrg'_0_1_0_1.
+                 injection IH_sstrg'_0_1_0_1 as IH_sstrg'_0_1_0_1.
+                 injection H_map_o_sstrg_1_1 as H_map_o_sstrg_1_1.
+                 rewrite H_map_o_sstrg_1_1 in IH_sstrg'_0_1_0_1.
+                 rewrite <- Heqstrg_w_v in IH_sstrg'_0_1_0_1.
+                 unfold concrete_interpreter.ConcreteInterpreter.sload in IH_sstrg'_0_1_0_1.
+                 rewrite not_eq_keys_snd_0 in IH_sstrg'_0_1_0_1.
+                 rewrite IH_sstrg'_0_1_0_1.
+                 reflexivity.
+        ** rewrite <- H_basic_sload_solver in H_add_to_smap.
+           exists idx1.
+           exists m1.
+           split.
+           *** apply H_add_to_smap.
+           *** intros stk mem strg ctx H_stk_len.
+               destruct m.
+               simpl in H_add_to_smap.
+               injection H_add_to_smap as H_idx1 H_m1.
+               rewrite <- H_idx1.
+               rewrite <- H_m1.
+               simpl.
+               unfold eval_sstack_val.
+
+               assert(H_valid_ext_bindings: valid_bindings instk_height (S maxid) ((maxid, SymSLOAD skey (U_SSTORE sstack_val key value :: sstrg')) :: bindings) ops). simpl. split; auto.
+               
+               pose proof (eval_sstack_val'_succ (S (S maxid)) instk_height (FreshVar maxid) stk mem strg ctx (S maxid) ((maxid, SymSLOAD skey (U_SSTORE sstack_val key value :: sstrg')) :: bindings) ops (eq_sym H_stk_len) (Nat.lt_succ_diag_r maxid) H_valid_ext_bindings (gt_Sn_n (S maxid))) as H_eval_FV_maxid.
+               destruct  H_eval_FV_maxid as [v  H_eval_FV_maxid].
+               exists v.
+               rewrite H_eval_FV_maxid.
+               split; reflexivity.
+  Qed.
+
+  Lemma basic_sstorage_updater_remove_dups_valid:
+    forall sstack_val_cmp skey instk_height m ops sstrg sstrg_r,
+      symbolic_state_cmp.SymbolicStateCmp.safe_sstack_val_cmp_ext_1 sstack_val_cmp ->
+      valid_sstack_value instk_height (get_maxidx_smap m) skey ->
+      valid_sstorage instk_height (get_maxidx_smap m) sstrg ->
+      basic_sstorage_updater_remove_dups sstack_val_cmp skey sstrg instk_height m ops = sstrg_r ->
+      valid_sstorage instk_height (get_maxidx_smap m) sstrg_r.
+  Proof.
+    intros sstack_val_cmp skey instk_height m ops.
+    induction sstrg as [| u sstrg' IHsstrg'].
+    + intros sstrg_r H_sstack_val_cmp_snd H_valid_skey H_valid_sstrg H_basic_sstorage_updater_remove_dups.
+      simpl in H_basic_sstorage_updater_remove_dups.
+      rewrite <- H_basic_sstorage_updater_remove_dups.
+      reflexivity.
+    + intros sstrg_r H_sstack_val_cmp_snd H_valid_skey H_valid_sstrg H_basic_sstorage_updater_remove_dups.
+      unfold basic_sstorage_updater_remove_dups in H_basic_sstorage_updater_remove_dups.
+      fold basic_sstorage_updater_remove_dups in H_basic_sstorage_updater_remove_dups.
+      destruct u as [skey' svalue] eqn:E_u.
+      destruct (sstack_val_cmp (S (get_maxidx_smap m)) skey skey' (get_maxidx_smap m) (get_bindings_smap m) (get_maxidx_smap m) (get_bindings_smap m) instk_height ops) eqn:E_cmp_skey_skey'.
+      ++ apply IHsstrg'.
+         +++ apply H_sstack_val_cmp_snd.
+         +++ apply H_valid_skey.
+         +++ apply H_valid_sstrg.
+         +++ apply H_basic_sstorage_updater_remove_dups.
+      ++ destruct (not_eq_keys skey skey' (get_maxidx_smap m) (get_bindings_smap m) instk_height ops) eqn:E_not_eq_keys.
+         +++ destruct sstrg_r as [|u_r sstrg_r']; try discriminate.
+             injection H_basic_sstorage_updater_remove_dups as H_u_r H_sstrg_r'.
+             simpl.
+             split.
+             ++++ rewrite <- H_u_r.
+                  simpl.
+                  split; apply H_valid_sstrg.
+             ++++ apply IHsstrg'.
+                  +++++ apply H_sstack_val_cmp_snd.
+                  +++++ apply H_valid_skey.
+                  +++++ apply H_valid_sstrg.
+                  +++++ apply H_sstrg_r'.
+         +++ rewrite <- H_basic_sstorage_updater_remove_dups.
+             simpl.
+             split; try split; apply H_valid_sstrg.
+  Qed.
       
-            
     
-      
-  Admitted.
-          
-        
-      
+
   Lemma basic_sstorage_updater_snd: sstorage_updater_ext_snd basic_sstorage_updater.
+    unfold sstorage_updater_ext_snd.
+    intros sstack_val_cmp H_sstack_val_cmp_snd.
+    unfold sstorage_updater_snd.
+    split.
+    (* Validity *)
+    + unfold sstorage_updater_valid_res.
+      intros m sstrg sstrg' u instk_height ops.
+      intros H_valid_sstrg H_valid_u H_basic_sstrg_updater.
+         unfold basic_sstorage_updater in H_basic_sstrg_updater.
+         destruct u as [skey svalue] eqn:E_u.
+         destruct sstrg' as [|u' sstrg'']; try discriminate.
+         injection H_basic_sstrg_updater as H_u' H_sstrg''.
+         rewrite <- H_u'.
+         simpl.
+         split; try split; try apply H_valid_u.
+         
+         apply basic_sstorage_updater_remove_dups_valid in H_sstrg''.
+      ++ apply H_sstrg''.
+      ++ apply H_sstack_val_cmp_snd.
+      ++ apply H_valid_u.
+      ++ apply H_valid_sstrg.
+    + admit.
+      
   Admitted.
 
 End StorageOpsSolversImplSoundness.
+
